src/tools/parallelcomposition/generaldeduction/interleavinggeneraldeductionScript.sml
@@ -265,6 +265,26 @@ val OUTL_INR_FUN_thm = new_axiom("OUTL_INR_FUN", ``
 ∀x n.
  OUTL (INR x) = n x``);
 
+val DedRelINL = new_axiom ("DedRelINL",
+                          ``∀(ded1:('pred1) tded) (MTrn1:('event1 + 'eventS, 'pred1, 'state1, 'symb) mtrel) (MTrn2:('event2 + 'eventS, 'pred2, 'state2, 'symb) mtrel) Sym P S1 S2 Sym' P' S1' S2' P'' t1 t2 x.
+                            (
+                          (MTrn1 (Sym,IMAGE OUTL P,S1) t1 (Sym',IMAGE OUTL P'',S1')) ∧
+                          (MTrn2 (Sym,IMAGE OUTR P,S2) t2 (Sym',IMAGE OUTR P'',S2')) ∧
+                          (ded1 (IMAGE OUTL P'') x))
+                             ⇒
+                             ((MTrn1 (Sym,IMAGE OUTL P,S1) t1 (Sym',IMAGE OUTL P'' ∪ {x},S1')) ∧
+                              (MTrn2 (Sym,IMAGE OUTR P,S2) t2 (Sym',IMAGE OUTR P'' ∪ {OUTR (INL x)},S2')))``);
+                              
+val DedRelINR = new_axiom ("DedRelINR",
+                          ``∀(ded2:('pred2) tded) (MTrn1:('event1 + 'eventS, 'pred1, 'state1, 'symb) mtrel) (MTrn2:('event2 + 'eventS, 'pred2, 'state2, 'symb) mtrel) Sym P S1 S2 Sym' P' S1' S2' P'' t1 t2 x.
+                            (
+                          (MTrn1 (Sym,IMAGE OUTL P,S1) t1 (Sym',IMAGE OUTL P'',S1')) ∧
+                          (MTrn2 (Sym,IMAGE OUTR P,S2) t2 (Sym',IMAGE OUTR P'',S2')) ∧
+                          (ded2 (IMAGE OUTR P'') x))
+                             ⇒
+                             ((MTrn1 (Sym,IMAGE OUTL P,S1) t1 (Sym',IMAGE OUTL P'' ∪ {OUTL (INR x)},S1')) ∧
+                              (MTrn2 (Sym,IMAGE OUTR P,S2) t2 (Sym',IMAGE OUTR P'' ∪ {x},S2')))``);
+                              
 val TranRelNil = new_axiom ("TranRelNil",
                             ``∀(MTrn:('event, 'pred, 'state , 'symb ) mtrel) v p s. MTrn (v,p,s) [] (v,p,s)``);
 val TranRelConfigEq = new_axiom ("TranRelConfigEq",
@@ -318,12 +338,21 @@ new_axiom ("TranRelSnocRevSync",
            ``∀(MTrn1:('event1 + 'eventS, 'pred1, 'state1, 'symb) mtrel) (MTrn2:('event2 + 'eventS, 'pred2, 'state2, 'symb) mtrel) Sym P S1 S2 Sym' P' S1' S2' t1 t2 e.
                                                                         ((MTrn1 (Sym,IMAGE OUTL P,S1) (SOME (INR e)::t1) (Sym',IMAGE OUTL P',S1')) ∧ (MTrn2 (Sym,IMAGE OUTR P,S2) (SOME (INR e)::t2) (Sym',IMAGE OUTR P',S2'))) ⇒ (∃Sym'' (P'':('pred1+'pred2) set) S1'' S2''. (MTrn1 (Sym,IMAGE OUTL P,S1) t1 (Sym'',IMAGE OUTL P'',S1'')) ∧ (MTrn1 (Sym'',IMAGE OUTL P'',S1'') [SOME (INR e)] (Sym',IMAGE OUTL P',S1')) ∧ (MTrn2 (Sym,IMAGE OUTR P,S2) t2 (Sym'',IMAGE OUTR P'',S2'')) ∧ (MTrn2 (Sym'',IMAGE OUTR P'',S2'') [SOME (INR e)] (Sym',IMAGE OUTR P',S2')))``);                                                                        
 
-val TranRelSnocRevSync =
+val TranRelSnocRevNone =
 new_axiom ("TranRelSnocRevNone",
            ``
            ∀(MTrn1:('event1 + 'eventS, 'pred1, 'state1, 'symb) mtrel) (MTrn2:('event2 + 'eventS, 'pred2, 'state2, 'symb) mtrel) Sym P S1 S2 Sym' P' S1' S2' t1 t2.
              ((MTrn1 (Sym,IMAGE OUTL P,S1) t1 (Sym',IMAGE OUTL P',S1')) ∧ (MTrn2 (Sym,IMAGE OUTR P,S2) t2 (Sym',IMAGE OUTR P',S2')))
              ⇒ (∃(P'':('pred1+'pred2) set). (∀(Ded1:('pred1) tded) (Ded2:('pred2) tded) (Ded3:('pred1 + 'pred2) tded) phi. (combineAllDed Ded1 Ded2 Ded3 P'' phi) ∧ P'=P''∪{phi}) ∧
+                                            (MTrn1 (Sym,IMAGE OUTL P,S1) t1 (Sym',IMAGE OUTL P'',S1')) ∧
+                                            (MTrn2 (Sym,IMAGE OUTR P,S2) t2 (Sym',IMAGE OUTR P'',S2')))``);
+
+val TranRelSnocRevNoneComp =
+new_axiom ("TranRelSnocRevNoneComp",
+           ``
+           ∀(MTrn1:('event1 + 'eventS, 'pred1, 'state1, 'symb) mtrel) (MTrn2:('event2 + 'eventS, 'pred2, 'state2, 'symb) mtrel) Sym P S1 S2 Sym' P' S1' S2' t1 t2.
+             ((MTrn1 (Sym,IMAGE OUTL P,S1) t1 (Sym',IMAGE OUTL P',S1')) ∧ (MTrn2 (Sym,IMAGE OUTR P,S2) t2 (Sym',IMAGE OUTR P',S2')))
+             ⇒ (∃(P'':('pred1+'pred2) set). (∀(Ded1:('pred1) tded) (Ded2:('pred2) tded) phi. ((composeDed Ded1 Ded2) P'' phi) ∧ P'=P''∪{phi})  ∧
                                             (MTrn1 (Sym,IMAGE OUTL P,S1) t1 (Sym',IMAGE OUTL P'',S1')) ∧
                                             (MTrn2 (Sym,IMAGE OUTR P,S2) t2 (Sym',IMAGE OUTR P'',S2')))``);
 
